lush/Crypto/BitOperations.lean
@@ -1,0 +1,23 @@
+namespace UInt64
+def toArrayBE (n : UInt64) : Array UInt8 :=
+  #[ (n >>> (8 * 7)).toUInt8
+   , (n >>> (8 * 6)).toUInt8
+   , (n >>> (8 * 5)).toUInt8
+   , (n >>> (8 * 4)).toUInt8
+   , (n >>> (8 * 3)).toUInt8
+   , (n >>> (8 * 2)).toUInt8
+   , (n >>> (8 * 1)).toUInt8
+   , (n >>> (8 * 0)).toUInt8
+  ]
+end UInt64
+
+namespace UInt32
+def toArrayBE (n : UInt32) : Array UInt8 :=
+  #[ (n >>> (8 * 3)).toUInt8
+   , (n >>> (8 * 2)).toUInt8
+   , (n >>> (8 * 1)).toUInt8
+   , (n >>> (8 * 0)).toUInt8
+  ]
+
+theorem size_toArrayBE (n : UInt32) : n.toArrayBE.size = 4 := by simp [toArrayBE]
+end UInt32
